

CONTROL SYSTEMS

HOMEWORK-1

BHUKYA SIDDHU
EE18BTECH11004

IITH

February 12, 2020



Question 33

Let the state-space representation of an LTI system be.

$$\dot{x}(t) = Ax(t) + Bu(t)$$

$$y(t) = Cx(t) + Du(t)$$

A, B, C are matrices, D is scalar, $u(t)$ is input to the system and $y(t)$ is output to the system. let

$$b_1 = \begin{bmatrix} 0 & 0 & 1 \end{bmatrix}$$

$$b_1^T = B$$

and $D=0$. Find A and C.

$$H(s) = \frac{1}{s^3 + 3s^2 + 2s + 1}$$

Solution

STATE MODEL

Let $U_1(t)$ and $U_2(t)$ are the inputs of the MIMO system and $y_1(t), y_2(t)$ are the output of the system and $x_1(t)$ and $x_2(t)$ are the state variables.

so output equation is,

$$y1(t) = C_{11} \times x1(t) + C_{12} \times x2(t) + d_{11} \times U1(t) + d_{12} \times U2(t) \quad (1)$$

$$y2(t) = C_{21} \times x1(t) + C_{22} \times x2(t) + d_{21} \times U1(t) + d_{22} \times U2(t) \quad (2)$$

$$\begin{bmatrix} y1(t) \\ y2(t) \end{bmatrix} = \begin{bmatrix} C_{11} & C_{12} \\ C_{21} & C_{22} \end{bmatrix} \times \begin{bmatrix} x1(t) \\ x2(t) \end{bmatrix} + \begin{bmatrix} d_{11} & d_{12} \\ d_{21} & d_{22} \end{bmatrix} \times \begin{bmatrix} U1(t) \\ U2(t) \end{bmatrix}$$

therefore $Y(t)=C.X(t)+D.U(t)$

$$\dot{x1}(t) = a_{11} \times x1(t) + a_{12} \times x2(t) + b_{11} \times U1(t) + b_{12} \times U2(t) \quad (3)$$

$$\dot{x2}(t) = a_{21} \times x1(t) + a_{22} \times x2(t) + b_{21} \times U1(t) + b_{22} \times U2(t) \quad (4)$$

$$\begin{bmatrix} \dot{x}_1(t) \\ \dot{x}_2(t) \end{bmatrix} = \begin{bmatrix} a_{11} & a_{12} \\ a_{21} & a_{22} \end{bmatrix} \times \begin{bmatrix} x_1(t) \\ x_2(t) \end{bmatrix} + \begin{bmatrix} b_{11} & b_{12} \\ b_{21} & b_{22} \end{bmatrix} \times \begin{bmatrix} U_1(t) \\ U_2(t) \end{bmatrix}$$

therefore $\dot{X}(t) = A.X(t) + B.U(t)$

FINDING TRANSFER FUNCTION

So, $\dot{X}(t) = A.X(t) + B.U(t)$ be equation 1

and $Y(t) = C.X(t) + D.U(t)$ be equation 2

by applying laplace transforms on both sides of equation 1

we get

$$S.X(S) - X(0) = A.X(S) + B.U(S)$$

$$S.X(S) - A.X(S) = B.U(S) + X(0)$$

$$(S I - A)X(S) = X(0) + B.U(S)$$

$$X(S) = X(0)([S I - A])^{-1} + B.([S I - A])^{-1}.U(S)$$

Laplace transform of equation 2 and sub $X(S)$

$$Y(S)=C.X(S)+D.U(S)$$

$$Y(S)=C.[X(0)([SI-A])^{-1} + B.([SI - A])^{-1}.U(S)] + D.U(S)$$

$$\text{If } X(0)=0$$

$$\text{then } Y(S)=C.[B.([SI-A])^{-1}.U(S)] + D.U(S)$$

$$\frac{Y(S)}{U(S)} = C.[B.([SI - A])^{-1}] + D = H(S)$$

As we know that

$$H(s) = \frac{Y(S)}{U(s)} = \frac{1}{s^3 + 3s^2 + 2s + 1}$$

$$\text{let } X(S) = \frac{U(S)}{\text{denominator}}$$

$$Y(S)=X(S) \times \text{numerotor}$$

$$s^3X(s) + 3s^2X(s) + 2sX(s) + X(s) = U(S)$$

$$X'''(t) + 3X''(t) + 2X'(t) + X(t) = U(t)$$

$$X(t)=x_1 \quad \text{and} \quad \dot{x}_n = x_{n+1}$$

$$\dot{X} = \dot{x}_1$$

$$\dot{X} = \dot{x}_1 = x_2$$

$$\ddot{X} = \ddot{x}_1 = \dot{x}_2 = x_3$$

$$\ddot{\ddot{X}} = \ddot{\ddot{x}}_1 = \ddot{\ddot{x}}_2 = \dot{x}_3$$

$$\dot{x}_3 = -x_1 - 2x_2 - 3x_3 + U$$

$$\dot{x}_1 = x_2, \quad \dot{x}_2 = x_3$$

$$\begin{bmatrix} \dot{x}_1 \\ \dot{x}_2 \\ \dot{x}_3 \end{bmatrix} = \begin{bmatrix} 0 & 1 & 0 \\ 0 & 0 & 1 \\ -1 & -2 & -3 \end{bmatrix} \times \begin{bmatrix} x_1 \\ x_2 \\ x_3 \end{bmatrix} + \begin{bmatrix} 0 \\ 0 \\ 1 \end{bmatrix} \times U$$

therefore $A = \begin{bmatrix} 0 & 1 & 0 \\ 0 & 0 & 1 \\ -1 & -2 & -3 \end{bmatrix}$

Since $Y(S)=X(S) \times \text{numerator}$

therefore $Y(S)=X(S)$; $Y(t)=X(t)$

$$Y = \begin{bmatrix} 1 & 0 & 0 \end{bmatrix} \times \begin{bmatrix} x_1 \\ x_2 \\ x_3 \end{bmatrix}$$

$$C = \begin{bmatrix} 1 & 0 & 0 \end{bmatrix}$$